Core/Eval/SmallStep.lean
@@ -15,15 +15,15 @@ namespace Core
 @[simp]
 def Term.is_data (v : DataConst) : Vec Term m -> Option (Vec Constructor m)
 | .nil => return .nil
-| .cons (.spctor (m := m) (n := n) (.data v') c t1 t2) xs => do
+| .cons (.spctor (m1 := m1) (m2 := m2) (n := n) (.data v') c t1 t2 t3) xs => do
   let zs <- Term.is_data v xs
-  let z : Constructor := ⟨c, m, t1, n, t2.to⟩
+  let z : Constructor := ⟨c, m1, t1, m2, t2, n, t3.to⟩
   if v == v'
   then some (z :: zs)
   else none
 | .cons _ _ => none
 
-def get_match (ctors : Vec Constructor m) (ps : Vec (Pattern m) n) : Option (Pattern m × Fin n) := ps.find (Pattern.match ctors)
+def get_match (ctors : Vec Constructor m) (ps : Vec (Pattern m) n) : Option (Fin n) := ps.findIdx? (Pattern.match ctors)
 
 @[simp]
 def eval (G : List Global) : Term ->  Option Term
@@ -34,7 +34,7 @@ def eval (G : List Global) : Term ->  Option Term
 | .tbind _ _ _ => none
 | .lam _ _ => none
 | .ctor0 _ => none
-| .spctor (.data _) _ _ _ => none
+| .spctor (.data _) _ _ _ _ => none
 
 ----------------------------------------------------------------
 ---- Normal forms
@@ -48,35 +48,35 @@ def eval (G : List Global) : Term ->  Option Term
   let (_, t) <- lookup_defn G x
   return t
 
-| .spctor (n := n) .openm x Ts ss => do
-  let m_ss : Lilac.Fun.Vec (Option Term) n := λ i => eval G (ss i)
-  match (m_ss.to).find Option.isSome with
+| .spctor (n := n) .openm x Ts1 Ts2 ss => do
+  let m_ss : Vec (Option Term) n := Fun.Vec.to (λ i => eval G (ss i))
+  match (m_ss).findIdx? Option.isSome with
   | none =>
     let ctors <- Term.is_data .opn ss.to
-    let ⟨m, p, b⟩ <- get_instance x ctors G
-    let τ := Sequ.append_vec (Vec.map su Ts) +0
+    let ⟨_, _, b⟩ <- get_instance x ctors G
+    let τ := Ts1.list.map su ++ Ts2.list.map su ++ Subst.id Ty
     let σ := Constructor.subst ctors
-    return b[τ:Ty][σ]
-  | some (t', i) => do
-    let t' <- t'
-    return (.spctor .openm x Ts (ss.update t' i))
+    return b[τ][σ]
+  | some i => do
+    let t' <- eval G (ss i)
+    return (.spctor .openm x Ts1 Ts2 (ss.to.set i t').to)
 
 
 | .mtch m n ss ps bs => do
-  let m_ss : Lilac.Fun.Vec (Option Term) m := λ i => eval G (ss i)
-  match (m_ss.to).find Option.isSome with
+  let m_ss : Vec (Option Term) m := Fun.Vec.to (λ i => eval G (ss i))
+  match (m_ss).findIdx? Option.isSome with
   | none =>
     let ctors <- Term.is_data .cls ss.to
     let σ := Constructor.subst ctors
-    let ⟨_, i⟩ <- get_match ctors ps.to
+    let i <- get_match ctors ps.to
     return (bs i)[σ]
-  | some (t', i) => do
-    let t' <- t'
-    return (.mtch m n (ss.update t' i) ps bs)
+  | some i => do
+    let t' <- eval G (ss i)
+    return (.mtch m n (ss.to.set i t').to ps bs)
 
 -- Λ reduction
 | .ctor1 (.appt ty) (.tbind .lamt _ tm) => do
-  return (tm[su ty::+0:Ty])
+  return (tm[su ty::+0σ])
 | .ctor1 (.appt ty) t => do
   let t' <- eval G t
   return (.ctor1 (.appt ty) t')
@@ -84,14 +84,14 @@ def eval (G : List Global) : Term ->  Option Term
 
 -- λ reduction
 | .ctor2 .app (.lam _ t) t2 => do
-  return t[su t2::+0:Term]
+  return t[su t2::+0σ]
 | .ctor2 .app t1 t2 => do
   let t1' <- eval G t1
   return (.ctor2 .app t1' t2)
 
 -- ∀c
 | .ctor2 .apptc (.tbind .allc _ (.ctor0 (.refl (Ty.all _ t1)))) (.ctor0 (.refl t2)) => do
-  return .ctor0 (.refl t1[su t2::+0:Ty])
+  return .ctor0 (.refl t1[su t2::+0σ])
 | .ctor2 .apptc t1 t2 => do
    match eval G t1 with
    | none => match eval G t2 with
