Core/Examples/Boolean.lean
@@ -14,12 +14,12 @@ namespace Core.Examples
 /- data Bool = True | False -/
 def BoolCtx : GlobalEnv := [
   Global.data 2 "Bool" ★
-             #𝓋[ ("True", ⟨0, #𝓋[], 0, #𝓋[], gt#"Bool"⟩)
-               , ("False", ⟨0, #𝓋[], 0, #𝓋[], gt#"Bool"⟩)]
+             #( ("True", ⟨0, #(), 0, #(), 0, #(), gt#"Bool"⟩)
+               , ("False", ⟨0, #(), 0, #(), 0, #(), gt#"Bool"⟩))
   ]
 
-def TrueCtor : Term := ctor! "True" #𝓋[] .nil
-def FalseCtor : Term := ctor! "False" #𝓋[] .nil
+def TrueCtor : Term := ctor! "True" #() #() .nil
+def FalseCtor : Term := ctor! "False" #() #() .nil
 
 #guard TrueCtor.infer_type BoolCtx [] [] == .some gt#"Bool"
 #guard GlobalEnv.wf_globals [] == some ()
@@ -32,9 +32,9 @@ not = λ x → case x of
                True → False
 -/
 def notTerm : Core.Term := λ[  gt#"Bool" ]
-  mtch' #𝓋[#0]
-     #𝓋[ (#𝓋[⟨"True", 0,  #𝓋[] , 0⟩] , TrueCtor)
-       , (#𝓋[⟨"False", 0 , #𝓋[] , 0⟩] , FalseCtor) ]
+  mtch' #(#0)
+     #( (#(⟨"True", 0,  #(), 0, 0⟩) , TrueCtor)
+      , (#(⟨"False", 0 , #(), 0, 0⟩) , FalseCtor) )
 
 #guard Term.infer_type BoolCtx [] [] notTerm == some (gt#"Bool" -:> gt#"Bool")
 
@@ -48,18 +48,18 @@ def notTerm : Core.Term := λ[  gt#"Bool" ]
                        False → True
  -/
 def eqBool : Term := λ[ gt#"Bool" ] λ[ gt#"Bool" ]
-  (mtch' #𝓋[#1]
-     #𝓋[ (#𝓋[⟨"True", 0 , #𝓋[] , 0⟩]  ,
-          (mtch' #𝓋[#0]
-                 #𝓋[ (#𝓋[ ⟨"True", 0 , #𝓋[] , 0⟩ ], TrueCtor)
-                   , (#𝓋[ ⟨"False", 0 , #𝓋[] , 0⟩ ] , FalseCtor)
-                   ]))
+  (mtch' #(#1)
+     #( (#(⟨"True", 0 , #() , 0, 0⟩)  ,
+          (mtch' #(#0)
+                 #( (#( ⟨"True", 0 , #() , 0, 0⟩ ), TrueCtor)
+                   , (#( ⟨"False", 0 , #() , 0, 0⟩ ) , FalseCtor))
+                   ))
 
-       , (#𝓋[⟨"False", 0 , #𝓋[] , 0⟩]  ,
-          (mtch' #𝓋[#0]
-                 #𝓋[ (#𝓋[ ⟨"True", 0 , #𝓋[] , 0⟩ ], FalseCtor)
-                   , (#𝓋[ ⟨"False", 0 , #𝓋[] , 0⟩ ] , TrueCtor)
-                   ]))])
+       , (#(⟨"False", 0 , #(), 0, 0⟩)  ,
+          (mtch' #(#0)
+                 #( (#( ⟨"True", 0 , #() , 0, 0⟩ ), FalseCtor)
+                   , (#( ⟨"False", 0 , #() , 0, 0⟩ ) , TrueCtor)
+                   )))))
 
 #guard Term.infer_type BoolCtx [] [] eqBool == some (gt#"Bool" -:> (gt#"Bool" -:> gt#"Bool"))
 
@@ -69,7 +69,7 @@ def EqBoolCtx : GlobalEnv := [
   --    If EqBool[t] t~Bool ← i
   --        let c = refl @ tBool @ (refl @ tBool @ refl) in
   --        λb1. λb2. ==@Bool ▹ sym c
-  .inst "eq" #𝓋[⟨"EqBool", 1, #𝓋[t#0], 1⟩] (λ[ t#0 ] λ[ t#0 ] -- #2 t ~ Bool
+  .inst "eq" #(⟨"EqBool", 1, #(t#0), 0, 1⟩) (λ[ t#0 ] λ[ t#0 ] -- #2 t ~ Bool
         (((d#"eqBool" • (.cast t#0 #2 #1)) • (.cast t#0 #2 #0))) ),
 
   -- .defn "test" (∀[★] λ [t#0 ~[★]~ gt#"Bool"] λ[ t#0 ] λ[ t#0 ])
@@ -78,10 +78,10 @@ def EqBoolCtx : GlobalEnv := [
   .defn "eqBool" (gt#"Bool" -:> gt#"Bool" -:> gt#"Bool") eqBool,
 
   -- -- EqBool : ∀ t. t ~ Bool → Eq t
-  .octor "EqBool" ⟨1, #𝓋[★], 1 , #𝓋[t#0 ~[★]~ gt#"Bool"], (gt#"Eq" • t#0)⟩ ,
+  .octor "EqBool" ⟨1, #(★), 0, #(), 1 , #((t#0 ~[★]~ gt#"Bool")), (gt#"Eq" • t#0)⟩ ,
 
   -- -- == : ∀ t. Eq t → t → t → Bool
-  .openm "eq" ⟨1, #𝓋[★], 1, #𝓋[gt#"Eq" • t#0], t#0 -:> t#0 -:> gt#"Bool"⟩ ,
+  .openm "eq" ⟨1, #(★), 0, #(), 1, #(gt#"Eq" • t#0), t#0 -:> t#0 -:> gt#"Bool"⟩ ,
 
   -- class Eq a
   .odata "Eq" (★ -:> ★),
@@ -96,12 +96,12 @@ def EqBoolCtx : GlobalEnv := [
 #eval ((d#"eqBool" • TrueCtor) • TrueCtor).eval_loop EqBoolCtx
 #eval ((d#"eqBool" • TrueCtor) • FalseCtor).eval_loop EqBoolCtx
 
-def iBool : Term := inst! "EqBool" #𝓋[ gt#"Bool" ] (Vec.to #𝓋[ refl! gt#"Bool"])
+def iBool : Term := inst! "EqBool" #( gt#"Bool" ) #() (Vec.to #( refl! gt#"Bool"))
 #guard iBool.infer_type EqBoolCtx [] [] == some (gt#"Eq" • gt#"Bool")
 
 -- #eval get_instance "EqBool" ((#𝓋[ iBool ])) EqBoolCtx
 
-def t1 : Term := ((openm! "eq" #𝓋[ gt#"Bool" ] (Vec.to (#𝓋[ iBool ]))) • TrueCtor) • FalseCtor
+def t1 : Term := ((openm! "eq" #( gt#"Bool" ) #() (Vec.to (#( iBool )))) • TrueCtor) • FalseCtor
 #guard t1.infer_type EqBoolCtx [] [] == some (gt#"Bool")
 -- def t2 : Term := (g#"eq" •[ gt#"Bool" ]  • (g#"EqBool" •[  gt#"Bool" ] • refl! gt#"Bool") • g#"True") • g#"True"
 
@@ -111,10 +111,10 @@ def t1 : Term := ((openm! "eq" #𝓋[ gt#"Bool" ] (Vec.to (#𝓋[ iBool ]))) •
 -- #eval! (Λ[★] λ[(t#0 ~[★]~ gt#"Bool")] λ[t#0] λ[t#0]
 --              (((d#"eqBool" • (.cast t#0 #2 #1)) • (.cast t#0 #2 #0)))).infer_type EqBoolCtx [] []
 
-def t2 : Term := ((openm! "eq" #𝓋[ gt#"Bool" ] (Vec.to (#𝓋[ iBool ]))) • TrueCtor) • TrueCtor
+def t2 : Term := ((openm! "eq" #( gt#"Bool") #() (Vec.to (#(iBool)))) • TrueCtor) • TrueCtor
 #eval t2.eval_loop EqBoolCtx
 
-def t3 : Term := ((openm! "eq" #𝓋[ gt#"Bool" ] (Vec.to (#𝓋[ iBool ]))) • TrueCtor) • FalseCtor
+def t3 : Term := ((openm! "eq" #( gt#"Bool") #() (Vec.to (#(iBool)))) • TrueCtor) • FalseCtor
 #eval t3.eval_loop EqBoolCtx
 
 
