Core/Infer/TypeSound.lean
@@ -15,12 +15,14 @@ namespace Core
 
 
 theorem pattern_binders_sound {G : GlobalEnv} {Δ : KindEnv} {m : Nat} {Ts : Vec Ty m} {p : Pattern m}:
-  pattern_binders G Δ m Ts p = some Γ ->
-  PatternBinders G Δ m Ts p Γ := by
+  pattern_binders G Δ m Ts p = some (Δ', Γ) ->
+  PatternBinders G Δ m Ts p Δ' Γ := by
 intro h
-induction m generalizing Γ <;> simp at *
+induction m generalizing Γ Δ' <;> simp at *
 case _ =>
   cases Ts; cases p; cases h
+  case _ e1 e2 =>
+  subst e1; subst e2
   apply PatternBinders.zero
 case _ n ih =>
   cases Ts; case _ T S =>
@@ -33,30 +35,29 @@ case _ n ih =>
   rw[Option.bind_eq_some_iff] at h; rcases h with ⟨Ks, h6, h⟩; simp at h
   rcases h with ⟨h7, h8, h9⟩
   replace ih := ih h2
-  have lem' := Vec.eq_sound' h7;
 
-  replace h6 := Vec.seq_sound_get_elem h6
-  simp only [<-h5.2] at Ks
-  simp [SpineTy] at h3;
-  let Ts := h3.2.2.2.fst
-  let Ts'' := Vec.map (fun T => T[Sequ.append_vec (Vec.map LeanSubst.su p.2.2.fst) +0:_]) Ts
-  let R := h3.2.2.2.2
-  let As := p.2.2.fst
-  rw[<-h5.2] at As
-  let R' := R[Sequ.append_vec (Vec.map su As) +0:Ty]
-  generalize c_def : p.fst = c at *
-  let na := p.2.fst
-  let na' := h3.1
-  let nb := p.2.2.2
-  let nb' := h3.2.2.1
-  let h := @PatternBinders.succ G Δ h3.snd.snd.1 c h3.1 Ks (S := S) (p := ps') (ℓ := Γ') (R := R) (As := As) (R' := R') (Ts := Ts) (Ts' := Ts'') n
-    (by have lem : Ks = h3.2.1 := by sorry
-        simp[h4, Ts, R, lem])
-    (by intro i; rw[h5.2] at i; replace h6 := h6 i; sorry)
-    (by unfold Ts''; sorry)
-    (by unfold R'; rfl) ih
-  subst h9; subst h8;
-  simp at h; unfold R' at h; unfold R at h
+  replace h6 := Vec.map_seq_sound _ h6
+  -- simp only [<-h5.2] at Ks
+  -- simp [SpineTy] at h3;
+  -- let Ts := h3.2.2.2.fst
+  -- let Ts'' := Vec.map (fun T => T[Sequ.append_vec (Vec.map LeanSubst.su p.2.2.fst) +0:_]) Ts
+  -- let R := h3.2.2.2.2
+  -- let As := p.2.2.fst
+  -- rw[<-h5.2] at As
+  -- let R' := R[Sequ.append_vec (Vec.map su As) +0:Ty]
+  -- generalize c_def : p.fst = c at *
+  -- let na := p.2.fst
+  -- let na' := h3.1
+  -- let nb := p.2.2.2
+  -- let nb' := h3.2.2.1
+  -- let h := @PatternBinders.succ G Δ h3.snd.snd.1 c h3.1 Ks (S := S) (p := ps') (ℓ := Γ') (R := R) (As := As) (R' := R') (Ts := Ts) (Ts' := Ts'') n
+  --   (by have lem : Ks = h3.2.1 := by sorry
+  --       simp[h4, Ts, R, lem])
+  --   (by intro i; rw[h5.2] at i; replace h6 := h6 i; sorry)
+  --   (by unfold Ts''; sorry)
+  --   (by unfold R'; rfl) ih
+  -- subst h9; subst h8;
+  -- simp at h; unfold R' at h; unfold R at h
 
   sorry
 
@@ -95,58 +96,36 @@ theorem data_valid_sound (G : GlobalEnv) :
   T.data? c G := by
 intro h
 induction T <;> simp [Ty.valid_data] at *
-case _ =>
-  rw[Option.bind_eq_some_iff] at h; rcases h with ⟨h1, h2, h⟩
-  simp at h;
-  simp [Ty.data?, Ty.HeadVariable];
-  exists h1.fst
-case _ =>
-  rw[Option.bind_eq_some_iff] at h; rcases h with ⟨h1, h2, h⟩
-  simp at h;
-  simp [Ty.data?, Ty.HeadVariable];
-  exists h1.fst
-  apply And.intro
-  · exists h1.2;
-  · apply h
-case _ a h _ =>
-  rw[Option.bind_eq_some_iff] at h; rcases h with ⟨h1, h2, h⟩
-  simp at h;
-  simp [Ty.data?, Ty.HeadVariable];
-  exists h1.1
-  replace h2 := Ty.Spine.app_eq.1 h2;
-  rcases h2 with ⟨w, h2, h3⟩;
-  apply And.intro
-  · exists w ++ [a]; exists w;
-  · apply h
+all_goals (assumption)
 
 theorem spine_kinding_sound :
-  spine_kinding G v x spTy = some () ->
-  SpineKinding v x G spTy
+  spine_kinding G v x test spTy = some () ->
+  SpineKinding v x G test spTy
 := by
 intro h
 unfold spine_kinding at h; split at h; simp at h
-case _ Ks _ _ _ =>
+case _ Ks1 _ Ks _ _ _ =>
 rw[Option.bind_eq_some_iff] at h; rcases h with ⟨h1, h2, h⟩
 rw[Option.bind_eq_some_iff] at h; rcases h with ⟨h3, h4, h⟩
 simp at h; rcases h with ⟨h5, h⟩
 rcases h5 with ⟨h5, h6⟩; subst h6;
 split at h
 · simp at h;
-  apply SpineKinding.valid (Δ := Ks.to_list)
+  apply SpineKinding.valid (Δ := (Ks1.list ++ Ks.list).reverse)
   · rfl
   · intro i; replace h2 := Vec.map_seq_sound _ h2 i; replace h2 := infer_kind_sound h2;
-    replace h5 := Vec.elems_eq_to_sound h5 i; rw[h5] at h2; apply h2
-  · apply infer_kind_sound h4
-  · intros _ e; cases e; apply h
+    replace h5 := Vec.elems_eq_to_sound h5 i; rw[h5] at h2; simp; apply h2
+  · simp; apply infer_kind_sound h4
+  · apply h
   · intro h; cases h
 
 · rw[Option.bind_eq_some_iff] at h; rcases h with ⟨h6, h, _⟩
-  apply SpineKinding.valid (Δ := Ks.to_list)
+  apply SpineKinding.valid (Δ := (Ks1.list ++ Ks.list).reverse)
   · rfl
   · intro i; replace h2 := Vec.map_seq_sound _ h2 i; replace h2 := infer_kind_sound h2;
-    replace h5 := Vec.elems_eq_to_sound h5 i; rw[h5] at h2; apply h2
-  · apply infer_kind_sound h4
-  · intros _ e; cases e
+    replace h5 := Vec.elems_eq_to_sound h5 i; rw[h5] at h2; simp; apply h2
+  · simp; apply infer_kind_sound h4
+  · sorry
   · intro _ i; replace h := Vec.map_seq_sound _ h i
     apply data_valid_sound; replace h6 := Vec.units h6 i; rw[h6] at h
     apply h
@@ -178,81 +157,85 @@ case _ => -- defn
 
 case _ As _ ih => -- spctor
   rw[Option.bind_eq_some_iff] at h; rcases h with ⟨h1, h2, h⟩
-  rw[Option.bind_eq_some_iff] at h; rcases h with ⟨Ks, h4, h⟩; simp at h
-  rcases h with ⟨h5, h⟩
+  rw[Option.bind_eq_some_iff] at h; rcases h with ⟨Ks1, h4, h⟩;
+  rw[Option.bind_eq_some_iff] at h; rcases h with ⟨Ks, h5, h⟩;
+  simp at h; rcases h with ⟨h5, h⟩
   rw[Option.bind_eq_some_iff] at h; rcases h with ⟨Ts', h7, h⟩; simp at h
   rcases h with ⟨h8, h⟩
   rcases h8 with ⟨h9, h10⟩
   rcases h9 with ⟨h11, h12⟩
   subst h10;
-  rcases h5 with ⟨h5, e⟩; subst e
-  replace h5 := Vec.eq_sound_lem h5; subst Ks
-  replace h12 := Vec.eq_sound_lem h12
-  apply Typing.spctor (R := h1.2.2.2.snd) (Ts := h1.2.2.2.1) (Ks := h1.2.1) (Ts' := Ts')
-  · rw[h2]
-  · apply Eq.symm h12
-  · apply Eq.symm h
-  · intro i; replace h4 := Vec.map_seq_sound _ h4 i; replace h4 := infer_kind_sound h4;
-    simp[instGetElem_Vec]; apply h4
-  · intro i; replace h7 := Vec.seq_sound1 _ h7 i;
-    apply ih i; simp[instGetElem_Vec]; rw[Vec.to_get_elem] at h7; apply h7
-  · intro c e; cases e; apply h11
-  · intro h; cases h
+  -- rcases h5 with ⟨e1, ⟨e2, ⟨e3, h5⟩⟩⟩
+  -- rcases e0 with ⟨e0, e6⟩
 
+  -- replace h5 := Vec.eq_sound_lem h5; subst Ks
+  -- replace h12 := Vec.eq_sound_lem h12
+  -- apply Typing.spctor (R := h1.2.2.2.snd) (Ts := h1.2.2.2.1) (Ks := h1.2.1) (Ts' := Ts')
+  -- · rw[h2]
+  -- · apply Eq.symm h12
+  -- · apply Eq.symm h
+  -- · intro i; replace h4 := Vec.map_seq_sound _ h4 i; replace h4 := infer_kind_sound h4;
+  --   simp[instGetElem_Vec]; apply h4
+  -- · intro i; replace h7 := Vec.seq_sound1 _ h7 i;
+  --   apply ih i; simp[instGetElem_Vec]; rw[Vec.to_get_elem] at h7; apply h7
+  -- · intro c e; cases e; apply h11
+  -- · intro h; cases h
+  sorry
 
 case _ As _ ih => -- openm
   rw[Option.bind_eq_some_iff] at h; rcases h with ⟨h1, h2, h⟩
-  rw[Option.bind_eq_some_iff] at h; rcases h with ⟨Ks, h4, h⟩
+  rw[Option.bind_eq_some_iff] at h; rcases h with ⟨Ks1, h4, h⟩
+  rw[Option.bind_eq_some_iff] at h; rcases h with ⟨Ks, h5, h⟩
   simp at h; rcases h with ⟨h5, h⟩
   rw[Option.bind_eq_some_iff] at h; rcases h with ⟨Ts', h7, h⟩
   rw[Option.bind_eq_some_iff] at h; rcases h with ⟨h8, h9, h⟩
   simp at h; rcases h with ⟨h10, h11⟩
   rcases h10 with ⟨h10, e⟩; subst e
   rcases h5 with ⟨h5, e⟩; subst e
-  replace h5 := Vec.eq_sound_lem h5; subst Ks
-  replace h12 := Vec.eq_sound_lem h10
-  apply Typing.spctor (R := h1.2.2.2.snd) (Ts := h1.2.2.2.1) (Ks := h1.2.1) (Ts' := Ts')
-  · rw[h2]
-  · apply Eq.symm h12
-  · apply Eq.symm h11
-  · intro i; replace h4 := Vec.map_seq_sound _ h4 i; replace h4 := infer_kind_sound h4;
-    simp[instGetElem_Vec]; apply h4
-  · intro i; replace h7 := Vec.seq_sound1 _ h7 i;
-    apply ih i; simp[instGetElem_Vec]; rw[Vec.to_get_elem] at h7; apply h7
-  · intro c e; cases e
-  · intro e i; cases e; replace h9 := Vec.map_seq_sound _ h9 i;
-    have lem := Vec.units h8 i; rw[lem] at h9
-    replace h9 := data_valid_sound _ h9; simp[instGetElem_Vec];
-    apply h9
-
+  -- replace h5 := Vec.eq_sound_lem h5; subst Ks
+  -- replace h12 := Vec.eq_sound_lem h10
+  -- apply Typing.spctor (R := h1.2.2.2.snd) (Ts := h1.2.2.2.1) (Ks := h1.2.1) (Ts' := Ts')
+  -- · rw[h2]
+  -- · apply Eq.symm h12
+  -- · apply Eq.symm h11
+  -- · intro i; replace h4 := Vec.map_seq_sound _ h4 i; replace h4 := infer_kind_sound h4;
+  --   simp[instGetElem_Vec]; apply h4
+  -- · intro i; replace h7 := Vec.seq_sound1 _ h7 i;
+  --   apply ih i; simp[instGetElem_Vec]; rw[Vec.to_get_elem] at h7; apply h7
+  -- · intro c e; cases e
+  -- · intro e i; cases e; replace h9 := Vec.map_seq_sound _ h9 i;
+  --   have lem := Vec.units h8 i; rw[lem] at h9
+  --   replace h9 := data_valid_sound _ h9; simp[instGetElem_Vec];
+  --   apply h9
+  sorry
 case _ m n ss ps ts smτs ih1 ih2 => -- match
   rw[Option.bind_eq_some_iff] at h; rcases h with ⟨S, h2, h⟩
   rw[Option.bind_eq_some_iff] at h; rcases h with ⟨h3, h4, h⟩
   rw[Option.bind_eq_some_iff] at h; rcases h with ⟨ξ, h6, h⟩
   rw[Option.bind_eq_some_iff] at h; rcases h with ⟨h7, h8, h⟩
   rw[Option.bind_eq_some_iff] at h; rcases h with ⟨h9, h10, h11⟩
-  apply Typing.mtch (m := m) (n := n) (S := S.to) (ξ := ξ.to)
-  · intro i; unfold smτs at h2; replace h2 := Vec.seq_sound1 _ h2;
-    apply ih1 i (T := S.to i) (h2 i);
-  · intro i; replace h4 := Vec.map_seq_sound _ h4 i;
-    have lem := Vec.units h3 i; rw[lem] at h4
-    rw[Vec.to_get_elem]
-    apply data_valid_sound _ h4
-  · intro i; replace h6 := Vec.seq_sound1 _ h6 i;
-    apply pattern_binders_sound;
-    rw[<-Fun.Vec.to_iso (v := S)] at h6; apply h6
-  · intro i; replace ih2 := ih2 ξ;
-    replace ih2 := ih2 (T := T) i
-    rw[Vec.get_elem_indexing (vs := ξ)]
-    apply ih2
-    replace h10 := Vec.seq_sound2 _ h10 i;
-    replace h11 := Vec.get_elem_if_eq_sound h11 i
-    rw[Vec.to_get_elem, h11] at h10; apply h10
-  · rw[<-Fun.Vec.to_iso (v := S)] at h8; intro q qs;
-    have lem := pattern_exhaustive_sound qs h8
-    rcases lem with ⟨i, lem⟩
-    exists i; rw[Fun.Vec.to_get_elem ps]; apply lem
-
+  -- apply Typing.mtch (m := m) (n := n) (S := S.to) (ξ := ξ.to)
+  -- · intro i; unfold smτs at h2; replace h2 := Vec.seq_sound1 _ h2;
+  --   apply ih1 i (T := S.to i) (h2 i);
+  -- · intro i; replace h4 := Vec.map_seq_sound _ h4 i;
+  --   have lem := Vec.units h3 i; rw[lem] at h4
+  --   rw[Vec.to_get_elem]
+  --   apply data_valid_sound _ h4
+  -- · intro i; replace h6 := Vec.seq_sound1 _ h6 i;
+  --   apply pattern_binders_sound;
+  --   rw[<-Fun.Vec.to_iso (v := S)] at h6; apply h6
+  -- · intro i; replace ih2 := ih2 ξ;
+  --   replace ih2 := ih2 (T := T) i
+  --   rw[Vec.get_elem_indexing (vs := ξ)]
+  --   apply ih2
+  --   replace h10 := Vec.seq_sound2 _ h10 i;
+  --   replace h11 := Vec.get_elem_if_eq_sound h11 i
+  --   rw[Vec.to_get_elem, h11] at h10; apply h10
+  -- · rw[<-Fun.Vec.to_iso (v := S)] at h8; intro q qs;
+  --   have lem := pattern_exhaustive_sound qs h8
+  --   rcases lem with ⟨i, lem⟩
+  --   exists i; rw[Fun.Vec.to_get_elem ps]; apply lem
+  sorry
 case _ ih1 ih2 => -- cast
   rw[Option.bind_eq_some_iff] at h; rcases h with ⟨h1, h2, h⟩
   rw[Option.bind_eq_some_iff] at h; rcases h with ⟨h3, h4, h⟩
